Cleanups of safety proof.  Next step is to augment patterns to include nonce checking

KeyManagement/Simulation.v
@@ -251,25 +251,25 @@ Section RealWorldUniverseProperties.
     end.
 
 
-  Inductive next_cmd_safe (honestk : key_perms) (cs : ciphers) (u_id : user_id) (sents : sent_nonces) :
+  Inductive next_cmd_safe (honestk : key_perms) (cs : ciphers) (u_id : user_id) (froms : recv_nonces) (sents : sent_nonces) :
     forall {A}, user_cmd A -> Prop :=
 
   | SafeBind : forall {r A} (cmd1 : user_cmd r) (cmd2 : r -> user_cmd A),
-      next_cmd_safe honestk cs u_id sents cmd1
-      -> next_cmd_safe honestk cs u_id sents (Bind cmd1 cmd2)
+      next_cmd_safe honestk cs u_id froms sents cmd1
+      -> next_cmd_safe honestk cs u_id froms sents (Bind cmd1 cmd2)
   | SafeEncrypt : forall {t} (msg : message t) k__sign k__enc msg_to,
       honestk $? k__enc = Some true
       -> (forall k_id kp, findKeysMessage msg $? k_id = Some kp -> honestk $? k_id = Some true)
-      -> next_cmd_safe honestk cs u_id sents (SignEncrypt k__sign k__enc msg_to msg)
+      -> next_cmd_safe honestk cs u_id froms sents (SignEncrypt k__sign k__enc msg_to msg)
   | SafeSign : forall {t} (msg : message t) k msg_to,
       (forall k_id kp, findKeysMessage msg $? k_id = Some kp -> honestk $? k_id = Some true /\ kp = false)
-      -> next_cmd_safe honestk cs u_id sents (Sign k msg_to msg)
+      -> next_cmd_safe honestk cs u_id froms sents (Sign k msg_to msg)
   | SafeRecv : forall t pat,
       msg_pattern_safe honestk pat
       (* /\ exists c_id c, msg = SignedCiphertext c_id *)
       (*           /\ cs $? c_id = Some c *)
       (*           /\ ~ List.In (cipher_nonce c) froms *)
-      -> next_cmd_safe honestk cs u_id sents (@Recv t pat)
+      -> next_cmd_safe honestk cs u_id froms sents (@Recv t pat)
   | SafeSend : forall {t} (msg : crypto t) msg_to,
         msg_honestly_signed honestk cs msg = true
       -> msg_to_this_user cs (Some msg_to) msg = true
@@ -278,14 +278,14 @@ Section RealWorldUniverseProperties.
                 /\ cs $? c_id = Some c
                 /\ fst (cipher_nonce c) = (Some u_id)  (* only send my messages *)
                 /\ ~ List.In (cipher_nonce c) sents)
-      -> next_cmd_safe honestk cs u_id sents (Send msg_to msg)
+      -> next_cmd_safe honestk cs u_id froms sents (Send msg_to msg)
   .
 
   Definition honest_cmds_safe {A B} (U : universe A B) : Prop :=
     forall u_id u honestk,
       honestk = findUserKeys U.(users)
       -> U.(users) $? u_id = Some u
-      -> next_cmd_safe (findUserKeys U.(users)) U.(all_ciphers) u_id u.(sent_nons) u.(protocol).
+      -> next_cmd_safe (findUserKeys U.(users)) U.(all_ciphers) u_id u.(from_nons) u.(sent_nons) u.(protocol).
 
   Definition label_safe (honestk : key_perms) (cs : ciphers) (lbl : label) : Prop :=
     match lbl with
@@ -359,48 +359,14 @@ Section Simulation.
         R (RealWorld.peel_adv U__r) U__i
       -> universe_ok U__r
       -> adv_universe_ok U__r
-      -> forall U__ra b,
-          U__r = strip_adversary_univ U__ra b
-          -> forall U__ra' lbl,
-            RealWorld.step_universe U__ra lbl U__ra'
-            -> label_safe (RealWorld.findUserKeys U__r.(RealWorld.users))
-                         U__r.(RealWorld.all_ciphers)
-                         lbl.
-
-  Definition honest_actions_safe' :=
-    forall (U__r : RealWorld.universe A B) U__i,
-        R (RealWorld.peel_adv U__r) U__i
-      -> universe_ok U__r
-      -> adv_universe_ok U__r
       -> honest_cmds_safe U__r.
-
-  (* Definition simulates_universe_ok := *)
-  (*   forall B (U__r : RealWorld.universe A B) U__i, *)
-  (*       R (strip_adversary U__r) U__i *)
-  (*     -> universe_ok U__r *)
-  (*     -> adv_universe_ok U__r *)
-  (*     -> forall U__r' lbl, *)
-  (*       RealWorld.step_universe U__r lbl U__r' *)
-  (*       -> universe_ok U__r'. *)
-
-  (* Definition simulates_labeled_step_safe := *)
-  (*   forall B (U__r : RealWorld.universe A B) U__i, *)
-  (*     R (strip_adversary U__r) U__i *)
-  (*     -> forall U__r' a, *)
-  (*       RealWorld.step_universe U__r (Messages.Action a) U__r' (* excludes adversary steps *) *)
-  (*       -> action_adversary_safe *)
-  (*           (RealWorld.findUserKeys U__r.(RealWorld.users)) *)
-  (*           U__r.(RealWorld.all_ciphers) *)
-  (*           a. *)
 
   Definition simulates (U__r : RealWorld.universe A B) (U__i : IdealWorld.universe A) :=
 
     (* conditions for simulation steps *)
     simulates_silent_step
   /\ simulates_labeled_step
-  /\ honest_actions_safe'
-  (* /\ simulates_universe_ok *)
-  (* /\ simulates_labeled_step_safe *)
+  /\ honest_actions_safe
 
   (* conditions for start *)
   /\ R (RealWorld.peel_adv U__r) U__i
